TreapNode.dfy
@@ -27,29 +27,29 @@ class TreapNode {
                        (forall y :: y in right.repr ==> y !in left.repr)))
   }
 
-  method insertNode(node: TreapNode?) 
+  method insertNode(node: TreapNode?)
     requires this.Valid()
     modifies this.repr
     decreases this.repr
   {
     if (node == null) {return;}
     if (node.key < this.key) {
-        // Go to the left
-        if (this.left == null) {
-            this.repr := this.repr + node.repr;
-            this.left := node;
-        } else {
-            this.left.insertNode(node);
-            // TODO: check priority
-        }
+      // Go to the left
+      if (this.left == null) {
+        this.repr := this.repr + node.repr;
+        this.left := node;
+      } else {
+        this.left.insertNode(node);
+        // TODO: check priority
+      }
     } else {
       if (this.right == null) {
-            this.repr := this.repr + node.repr;
-            this.right := node;
-        } else {
-            this.right.insertNode(node);
-            // TODO: check priority
-        }
+        this.repr := this.repr + node.repr;
+        this.right := node;
+      } else {
+        this.right.insertNode(node);
+        // TODO: check priority
+      }
     }
   }
   predicate IsLeaf()
